** (palloca_props.wf_State) proved that when a program reaches a promotable alloca that defines pid, [|pid|] is None.
This property is important to prove SAS/DSE: DSE memory simulations
do not consider promotable locations; SAS mem-simulations ignore
promotoable locations between a SAS pair. To set up the simulation, we
need to know which location can be ignored.

In mem2reg, we only promote allocas in the entry block, such allocas
only run once. So we can look up the current stack frames, find all
defined variables by promotable allocas, whose values are the ignored
locations. So, palloca_props.wf_State is sufficient for mem2reg.

In general, a dead-store-elimination pass can work for arbitrary heap or
stack allocations---that can be in non-entry blocks, say in a loop. In
that case, looking up the current program state cannot find all ignored
locations. There are at least 3 solutions to solve the problem:

Suppose a store to id0 is dead, 

1) we consider a set of ignored locations IGN w.r.t id0---any value in the
set is a value that the program assigned to id0. The invariant is 
  if the current state is S, for any v in IGN, 
  then there exists a S', S' reaches S /\ S' defines id0 to be v

2) define a variant of operational semantics whose local state is a map
  id -> option (list value)
  Here, one id can have values with different versions. The runtime only
uses the latest one, while proofs or analysis use versions to keep track
old values that have been overwritten.

We should prove this semantics implies the invariant like 1).
Say id0 maps to v0, v1, ..., vn-1, vn at prog state Sn,
then there exist S0 S1, ..., Sn-1 that construct an execution sequence
to Sn.

The semantics formalizes one difference between SSA and lambda-calculus.
In SSA, single-assignment is only static, while in lambda-calculus,
single-assignment is both static and dynamic by substituting code. The
version-like semantics actually records the effects of
variable-overwriting in SSA, and simulates the code copy in
lambda-calculus: In SSA, a variable can be redefined at runtime iff the
variable is in a loop; if we consider a loop as a local function, each
new version the semantics created for the variable is like the
substitution that the standard application rule does.

3) The problem is also caused by not distinguishing readable and
unreadable locations when defining mem-relations. Concretely, the
current memory relatioins consider all memory locations except ignored
ones, although some of them are not readable by any pointers. For
example, in the case, the old version of id0 cannot be loaded by other 
pointers. 

Therefore, if a memory simulation only condisers locations that can be
loaded by some accessible variables in the program, the problem might also 
be solved??

** After solving this problem, we found that the memory simulation of
DSE has a similar problem like the problem of SAS that we had already
solved (See r3826), which is the next mission.



git-svn-id: https://webdav.seas.upenn.edu/svn/sol/vol@3852 eef5ea85-cc2e-0410-bd84-0fae1f012da8

src3.0/Transforms/palloca_props.v
@@ -1740,4 +1740,614 @@ Proof.
   intros. simpl in H. unfold wf_use_at_head. auto.
 Qed.
 
+(***************************************************************************)
+(*           pid is not defined until the allocation in entry              *)
 
+(* 
+      ---------------------------------
+      |               cs0             |
+      ---------------------------------
+      | csa  | csb  | [palloca] | cs3 |
+      ---------------------------------
+      |      cs1    |                 |
+      ---------------------------------
+      |      |         cs             |
+      ---------------------------------        
+*)
+Definition before_palloca (pinfo:PhiInfo) (cs:cmds) : Prop :=
+match getEntryBlock (PI_f pinfo) with
+| Some (block_intro _ _ cs0 _) =>
+  forall cs1 cs3,
+  cs0 =
+    cs1 ++
+    insn_alloca (PI_id pinfo) (PI_typ pinfo) (PI_num pinfo) (PI_align pinfo) ::
+    cs3 ->
+  (exists csa, exists csb,
+    cs1 = csa ++ csb /\ 
+    cs = csb ++ 
+         insn_alloca (PI_id pinfo) (PI_typ pinfo) (PI_num pinfo) 
+           (PI_align pinfo) :: cs3)
+| _ => True
+end.
+
+Lemma before_palloca_cons: forall pinfo c cs l0 ps0 cs0 tmn0,
+  getEntryBlock (PI_f pinfo) =
+    Some (block_intro l0 ps0 (cs0++c::cs) tmn0) ->
+  before_palloca pinfo cs ->
+  before_palloca pinfo (c::cs).
+Proof.
+  unfold before_palloca.
+  intros. rewrite H in H0. rewrite H.
+  intros cs1 cs3 Heq.
+  assert (Heq':=Heq).
+  apply_clear H0 in Heq.
+  destruct Heq as [csa [csb [J1 J2]]]; subst.
+  assert (cs0 ++ [c] = csa) as J.
+    anti_simpl_env. auto.
+  subst.
+  exists cs0. exists (c::csb). simpl_env. split; auto.
+Qed.
+
+Definition wf_defs (pinfo:PhiInfo) (lc:@Opsem.GVsMap DGVs) : Prop :=
+lookupAL _ lc (PI_id pinfo) = None.
+
+Definition wf_ExecutionContext (pinfo:PhiInfo) (ec:Opsem.ExecutionContext) 
+  : Prop :=
+Opsem.CurFunction ec = PI_f pinfo ->
+getEntryBlock (PI_f pinfo) = Some (Opsem.CurBB ec) ->
+before_palloca pinfo (Opsem.CurCmds ec) ->
+wf_defs pinfo (Opsem.Locals ec).
+
+Fixpoint wf_ECStack (pinfo:PhiInfo) (ecs:Opsem.ECStack) : Prop :=
+match ecs with
+| nil => True
+| ec::ecs' => wf_ExecutionContext pinfo ec /\ wf_ECStack pinfo ecs'
+end.
+
+Definition wf_State (pinfo:PhiInfo) (S:Opsem.State) : Prop :=
+wf_ECStack pinfo (Opsem.ECS S).
+
+Lemma wf_defs_updateAddAL: forall pinfo lc' i1 gv1 (Hwfpi: WF_PhiInfo pinfo)
+  (HwfDef: wf_defs pinfo lc') (Hneq: i1 <> PI_id pinfo),
+  wf_defs pinfo (updateAddAL _ lc' i1 gv1).
+Proof.
+  intros. unfold wf_defs in *. intros.
+  rewrite <- lookupAL_updateAddAL_neq; auto.
+Qed.
+
+Lemma preservation_return : forall pinfo (HwfPI : WF_PhiInfo pinfo)
+  F B rid RetTy Result lc F' B' c' cs' tmn' lc' EC Mem als als' cfg
+  EC1 EC2
+  (EQ1:EC1 = {| Opsem.CurFunction := F;
+                Opsem.CurBB := B;
+                Opsem.CurCmds := nil;
+                Opsem.Terminator := insn_return rid RetTy Result;
+                Opsem.Locals := lc;
+                Opsem.Allocas := als |})
+  (EQ2:EC2 = {| Opsem.CurFunction := F';
+                Opsem.CurBB := B';
+                Opsem.CurCmds := c' :: cs';
+                Opsem.Terminator := tmn';
+                Opsem.Locals := lc';
+                Opsem.Allocas := als' |})
+  Mem' lc'' (H : Instruction.isCallInst c' = true)
+  (H1 : Opsem.returnUpdateLocals
+          (OpsemAux.CurTargetData cfg) c'
+            Result lc lc' (OpsemAux.Globals cfg) = ret lc'')
+  (Hwfcfg : OpsemPP.wf_Config cfg)  
+  (Hwfpp : OpsemPP.wf_State cfg
+           {| Opsem.ECS := EC1 :: EC2 :: EC;
+              Opsem.Mem := Mem |})
+  (HwfS1 : wf_State pinfo
+            {| Opsem.ECS := EC1 :: EC2 :: EC;
+               Opsem.Mem := Mem |}),
+  wf_State pinfo
+     {| Opsem.ECS :=
+             {| Opsem.CurFunction := F';
+                Opsem.CurBB := B';
+                Opsem.CurCmds := cs';
+                Opsem.Terminator := tmn';
+                Opsem.Locals := lc'';
+                Opsem.Allocas := als' |} :: EC;
+        Opsem.Mem := Mem' |}.
+Proof.
+  intros. subst. destruct cfg as [S [los nts] Ps gl fs].
+  destruct Hwfcfg as [_ [_ [HwfSystem HmInS]]].
+  destruct Hwfpp as 
+    [_ [_ 
+     [
+       [
+         [_ [HBinF1 [HFinPs1 [_ [_ [l2 [ps2 [cs2' Heq2]]]]]]]]
+         _
+       ]
+       _
+     ]
+    ]]; subst.
+  destruct HwfS1 as [Hinscope1 [Hinscope2 HwfECs]]. simpl.
+  fold wf_ECStack in HwfECs. simpl in *.
+  split; auto.
+    SSCase "wf_EC".
+    intros J1 J2 J3. simpl in J1, J2, J3. simpl. subst.
+    assert (before_palloca pinfo (c' :: cs')) as Hin.
+      eapply before_palloca_cons; eauto.
+    destruct_cmd c'; tinv H.
+    unfold wf_ExecutionContext in *. simpl in Hinscope1, Hinscope2.
+    unfold Opsem.returnUpdateLocals in H1.
+    remember (Opsem.getOperandValue (los,nts) Result lc gl) as R1.
+    destruct R1; tinv H1.
+    destruct n; inv H1.
+      apply Hinscope2; auto.
+
+      remember (lift_op1 DGVs (fit_gv (los, nts) t0) g t0) as R2.
+      destruct R2; inv H2.
+      apply wf_defs_updateAddAL; auto.
+        eapply WF_PhiInfo_spec10 in HBinF1; eauto using wf_system__uniqFdef.
+Qed.
+
+Lemma preservation_return_void : forall pinfo
+  (HwfPI : WF_PhiInfo pinfo)
+  F B rid lc F' B' c' cs' tmn' lc' EC Mem als als' cfg EC1 EC2
+  (EQ1:EC1 = {| Opsem.CurFunction := F;
+                Opsem.CurBB := B;
+                Opsem.CurCmds := nil;
+                Opsem.Terminator := insn_return_void rid;
+                Opsem.Locals := lc;
+                Opsem.Allocas := als |})
+  (EQ2:EC2 = {| Opsem.CurFunction := F';
+                Opsem.CurBB := B';
+                Opsem.CurCmds := c' :: cs';
+                Opsem.Terminator := tmn';
+                Opsem.Locals := lc';
+                Opsem.Allocas := als' |})
+  (Hwfcfg : OpsemPP.wf_Config cfg)
+  (Hwfpp : OpsemPP.wf_State cfg
+           {| Opsem.ECS := EC1 :: EC2 :: EC;
+              Opsem.Mem := Mem |})
+  Mem' (H : Instruction.isCallInst c' = true)
+  (HwfS1 : wf_State pinfo
+            {| Opsem.ECS := EC1 :: EC2 :: EC;
+               Opsem.Mem := Mem |}),
+  wf_State pinfo
+     {| Opsem.ECS :=
+             {| Opsem.CurFunction := F';
+                Opsem.CurBB := B';
+                Opsem.CurCmds := cs';
+                Opsem.Terminator := tmn';
+                Opsem.Locals := lc';
+                Opsem.Allocas := als' |} :: EC;
+        Opsem.Mem := Mem' |}.
+Proof.
+  intros. subst. destruct cfg as [S [los nts] Ps gl fs].
+  destruct Hwfcfg as [_ [_ [HwfSystem HmInS]]].
+  destruct Hwfpp as 
+    [_ [_ 
+     [
+       [
+         [_ [HBinF1 [HFinPs1 [_ [_ [l2 [ps2 [cs2' Heq2]]]]]]]]
+         _
+       ]
+       _
+     ]
+    ]]; subst.
+
+  destruct HwfS1 as [Hinscope1 [Hinscope2 HwfECs]]. simpl.
+  simpl in Hinscope1, Hinscope2, HwfECs.
+  fold wf_ECStack in HwfECs.
+
+  split; auto.
+    SSCase "wf_EC".
+    intros J1 J2 J3. simpl in J1, J2, J3. simpl. subst.
+    assert (before_palloca pinfo (c' :: cs')) as Hin.
+      eapply before_palloca_cons; eauto.
+    destruct_cmd c'; tinv H.
+    unfold wf_ExecutionContext in *. simpl in Hinscope1, Hinscope2.
+    auto.
+Qed.
+
+Lemma preservation_cmd_updated_case : forall (F : fdef)(B : block)
+  (lc : @Opsem.GVsMap DGVs)(gv3 : GVsT DGVs) (cs : list cmd) (tmn : terminator) 
+  id0 c0 Mem0 als ECs pinfo Mem1 als'
+  (HwfPI : WF_PhiInfo pinfo) (Hid : Some id0 = getCmdID c0) EC
+  (Heq: EC = {| Opsem.CurFunction := F;
+                Opsem.CurBB := B;
+                Opsem.CurCmds := c0 :: cs;
+                Opsem.Terminator := tmn;
+                Opsem.Locals := lc;
+                Opsem.Allocas := als |}) cfg
+  (Hwfpp : OpsemPP.wf_State cfg
+           {| Opsem.ECS := EC :: ECs;
+              Opsem.Mem := Mem0 |})
+  (HwfS1 : wf_State pinfo
+            {| Opsem.ECS := EC :: ECs;
+               Opsem.Mem := Mem0 |})
+  (Hneq :  F = PI_f pinfo -> id0 <> PI_id pinfo),
+  wf_State pinfo
+     {|
+     Opsem.ECS := {|
+            Opsem.CurFunction := F;
+            Opsem.CurBB := B;
+            Opsem.CurCmds := cs;
+            Opsem.Terminator := tmn;
+            Opsem.Locals := updateAddAL (GVsT DGVs) lc id0 gv3;
+            Opsem.Allocas := als' |} :: ECs;
+     Opsem.Mem := Mem1 |}.
+Proof.
+  intros. subst.
+  destruct cfg as [S [los nts] Ps gl fs].
+  destruct Hwfpp as 
+    [Hnonempty [
+     [Hreach1 [HBinF1 [HFinPs1 [_ [_ [l1 [ps1 [cs1' Heq1]]]]]]]]
+     [HwfEC0 HwfCall]
+    ]]; subst.
+  fold (@OpsemPP.wf_ECStack DGVs) in HwfEC0.
+  destruct HwfS1 as [Hinscope HwfECs]. simpl.
+  simpl in Hinscope, HwfECs.
+  fold wf_ECStack in HwfECs.
+  split; auto.
+    intros J1 J2 J3. simpl in J1, J2, J3. simpl. subst.
+    unfold wf_ExecutionContext in *. simpl in Hinscope.
+    eapply wf_defs_updateAddAL; eauto.
+    apply Hinscope; auto.
+      eapply before_palloca_cons; eauto.
+Qed.
+
+Lemma preservation_mem_updated_case : forall (F : fdef)(B : block)
+  (lc : @Opsem.GVsMap DGVs)(gv3 : GVsT DGVs) (cs : list cmd) (tmn : terminator) 
+  c0 Mem0 als Mem1 als' ECs pinfo EC
+  (Heq: EC = {| Opsem.CurFunction := F;
+                Opsem.CurBB := B;
+                Opsem.CurCmds := c0 :: cs;
+                Opsem.Terminator := tmn;
+                Opsem.Locals := lc;
+                Opsem.Allocas := als |}) cfg
+  (Hwfpp : OpsemPP.wf_State cfg
+           {| Opsem.ECS := EC :: ECs;
+              Opsem.Mem := Mem0 |})
+  (HwfS1 : wf_State pinfo
+            {| Opsem.ECS := EC :: ECs;
+               Opsem.Mem := Mem0 |}),
+  wf_State pinfo
+     {|
+     Opsem.ECS := {|
+            Opsem.CurFunction := F;
+            Opsem.CurBB := B;
+            Opsem.CurCmds := cs;
+            Opsem.Terminator := tmn;
+            Opsem.Locals := lc;
+            Opsem.Allocas := als' |} :: ECs;
+     Opsem.Mem := Mem1 |}.
+Proof.
+  intros. subst.
+  destruct cfg as [S [los nts] Ps gl fs].
+  destruct Hwfpp as 
+    [Hnonempty [
+     [Hreach1 [HBinF1 [HFinPs1 [_ [_ [l1 [ps1 [cs1' Heq1]]]]]]]]
+     [HwfEC0 HwfCall]
+    ]]; subst.
+  fold (@OpsemPP.wf_ECStack DGVs) in HwfEC0.
+  destruct HwfS1 as [Hinscope HwfECs]. simpl.
+  fold wf_ECStack in HwfECs.
+  split; auto.
+    intros J1 J2 J3. simpl in J1, J2, J3. simpl. subst.
+    apply Hinscope; auto. simpl.
+      eapply before_palloca_cons; eauto.
+Qed.
+
+Ltac destruct_ctx_other :=
+match goal with
+| Hwfcfg : OpsemPP.wf_Config ?cfg,
+  Hwfpp : OpsemPP.wf_State ?cfg _,
+  HwfS1 : wf_State _ _ |- _ =>
+  let l5:=fresh "l5" in
+  let ps5:=fresh "ps5" in
+  let cs5:=fresh "cs5" in
+  destruct Hwfcfg as [_ [Hwfgl0 [HwfSystem HmInS]]];
+  destruct Hwfpp as 
+    [Hnonempty [
+     [Hreach1 [HBinF1 [HFinPs1 [_ [_ [l5 [ps5 [cs5 Heq1]]]]]]]]
+     [HwfEC0 HwfCall]
+    ]]; subst;
+  fold (@OpsemPP.wf_ECStack DGVs) in HwfEC0;
+  destruct HwfS1 as [Hinscope HwfECs]; simpl;
+  simpl in Hinscope, HwfECs;
+  fold wf_ECStack in HwfECs
+end.
+
+(* go to typings_props *)
+Lemma entryBlock_has_no_pred: forall s m F B l0 l3 ps cs tmn
+  (HwfF: wf_fdef s m F) (Hentry:  getEntryBlock F = Some B) (Huniq:uniqFdef F)
+  (HBinF : blockInFdefB (block_intro l3 ps cs tmn) F = true)
+  (Hsucc : In l0 (successors_terminator tmn))
+  (Hlkup: lookupBlockViaLabelFromFdef F l0 = Some B),
+  False.
+Proof.
+  intros. 
+  destruct B as [l1 ps1 cs1 tmn1].
+  apply lookupBlockViaLabelFromFdef_inv in Hlkup; auto.
+  destruct Hlkup as [EQ HBinF']; subst.
+  destruct F as [fh bs]. 
+  simpl in HBinF. clear HBinF'.
+  eapply getEntryBlock_inv in Hentry; eauto.
+Qed.
+
+Ltac preservation_sBranch:=
+  destruct_ctx_other;
+  split; try solve [
+    auto |
+    intros J1 J2 J3; simpl in *; subst;
+    elimtype False;
+      match goal with
+      | H: Some _ = (if ?e then _ else _) |- _ => destruct e
+      | |- _ => idtac
+      end;
+      eapply entryBlock_has_no_pred; eauto using wf_system__wf_fdef,
+                                                 wf_system__uniqFdef;
+                                     simpl; auto
+  ].
+
+Ltac id_neq_pid_tac :=
+match goal with
+| |- _ <> PI_id _ =>
+     intros; subst;
+     match goal with
+     | HBinF1: blockInFdefB _ _ = true |- _ =>
+       eapply WF_PhiInfo_spec10 in HBinF1; eauto using wf_system__uniqFdef
+     end
+end.
+
+Ltac preservation_pure_cmd_updated_case := abstract
+  (eapply preservation_cmd_updated_case; eauto; try solve
+    [simpl; auto | destruct_ctx_other; intro; id_neq_pid_tac]).
+
+Lemma arguments_dont_define_pid: forall pinfo fa rt fid la va bs TD gvs lc
+  (HwfP: WF_PhiInfo pinfo)
+  (Huniq: uniqFdef (fdef_intro (fheader_intro fa rt fid la va) bs))
+  (Heq: fdef_intro (fheader_intro fa rt fid la va) bs = PI_f pinfo)
+  (Hinit: Opsem.initLocals TD la gvs = ret lc),
+  wf_defs pinfo lc.
+Proof.
+  intros.
+  unfold wf_defs.
+  remember (lookupAL (GVsT DGVs) lc (PI_id pinfo)) as R.
+  destruct R as [gv|]; auto.
+  symmetry_ctx.
+  eapply OpsemProps.In_initLocals__In_getArgsIDs in HeqR; eauto.
+  rewrite Heq in Huniq.
+  apply WF_PhiInfo_spec1 in HwfP; auto.
+  rewrite <- Heq in Huniq.
+  eapply IngetArgsIDs__lookupCmdViaIDFromFdef in Huniq; eauto.
+  congruence.
+Qed.
+
+Lemma WF_PhiInfo_spec13: forall pinfo l5 ps5 cs5 cs tmn t v align0
+  (HwfP: WF_PhiInfo pinfo) (Huniq: uniqFdef (PI_f pinfo))
+  (Hentry: 
+    getEntryBlock (PI_f pinfo) =
+    ret block_intro l5 ps5 
+          (cs5 ++ insn_alloca (PI_id pinfo) t v align0 :: cs) tmn),
+  t = PI_typ pinfo /\ v = PI_num pinfo /\ align0 = PI_align pinfo.
+Proof.
+  intros.
+  apply WF_PhiInfo_spec1 in HwfP; auto.
+  apply entryBlockInFdef in Hentry.
+  eapply IngetCmdsIDs__lookupCmdViaIDFromFdef in Hentry; 
+    eauto using in_middle.
+  simpl in Hentry.
+  uniq_result. auto.
+Qed.
+
+Lemma preservation : forall pinfo cfg S1 S2 tr
+  (Hwfcfg: OpsemPP.wf_Config cfg) (Hwfpp: OpsemPP.wf_State cfg S1) 
+  (HwfPI: WF_PhiInfo pinfo) (HsInsn: Opsem.sInsn cfg S1 S2 tr)
+  (HwfS1: wf_State pinfo S1), wf_State pinfo S2.
+Proof.
+  intros.
+  (sInsn_cases (induction HsInsn) Case); destruct TD as [los nts]; simpl HwfS1.
+
+Case "sReturn". abstract (eapply preservation_return; eauto; simpl; auto).
+Case "sReturnVoid". 
+  abstract (eapply preservation_return_void; eauto; simpl; auto).
+Case "sBranch". abstract preservation_sBranch.
+Case "sBranch_uncond". abstract preservation_sBranch.
+Case "sBop". preservation_pure_cmd_updated_case.
+Case "sFBop". preservation_pure_cmd_updated_case.
+Case "sExtractValue". preservation_pure_cmd_updated_case.
+Case "sInsertValue". preservation_pure_cmd_updated_case.
+Case "sMalloc". preservation_pure_cmd_updated_case.
+Case "sFree". abstract (eapply preservation_mem_updated_case; eauto).
+Case "sAlloca". 
+  assert ((F = PI_f pinfo -> id0 <> PI_id pinfo) \/
+          (F = PI_f pinfo -> id0 = PI_id pinfo)) as J. 
+    destruct (id_dec id0 (PI_id pinfo)); tauto.
+  destruct J as [J | J].
+    preservation_pure_cmd_updated_case.
+
+    abstract (
+    destruct_ctx_other;
+    split; try solve [
+      auto |
+      intros J1 J2 J3; simpl in J1, J2, J3; simpl; subst;
+      rewrite J in J2; auto;
+      unfold before_palloca in J3;
+      rewrite J2 in J3;
+      assert (uniqFdef (PI_f pinfo)) as Huniq; 
+        try solve [match goal with
+                   | |- uniqFdef _ => eauto using wf_system__uniqFdef
+                   end];
+      apply WF_PhiInfo_spec13 in J2; auto;
+      destruct J2 as [A [B C]]; subst;
+      destruct (@J3 cs5 cs) as [csa [csb [EQ1 EQ2]]]; auto;
+      anti_simpl_env
+    ]).
+Case "sLoad". preservation_pure_cmd_updated_case.
+Case "sStore". abstract (eapply preservation_mem_updated_case; eauto).
+Case "sGEP". preservation_pure_cmd_updated_case.
+Case "sTrunc". preservation_pure_cmd_updated_case.
+Case "sExt". preservation_pure_cmd_updated_case.
+Case "sCast". preservation_pure_cmd_updated_case.
+Case "sIcmp". preservation_pure_cmd_updated_case.
+Case "sFcmp". preservation_pure_cmd_updated_case.
+Case "sSelect". destruct (isGVZero (los, nts) c); preservation_pure_cmd_updated_case.
+Case "sCall".
+  abstract (
+  destruct_ctx_other;
+  split; try solve [
+    auto |
+    intros J1 J2 J3; simpl in J1, J2, J3; simpl;
+      apply OpsemAux.lookupFdefViaPtr_inv in H1; auto;
+      eapply arguments_dont_define_pid; eauto using wf_system__uniqFdef |
+    split; auto
+  ]).
+Case "sExCall". 
+  abstract( 
+  destruct_ctx_other;
+  split; try solve [
+    auto |
+    intros J1 J2 J3; simpl in J1, J2, J3; simpl; subst;
+    assert (wf_defs pinfo lc) as Hwd; try solve [
+      match goal with
+      | |- wf_defs _ _ =>
+        apply Hinscope; simpl; try solve 
+          [auto | eapply before_palloca_cons; eauto]
+      end
+    ];
+    unfold Opsem.exCallUpdateLocals in *;
+    destruct_if; try solve [
+      auto |
+      inv_mbind; try solve [
+       auto |
+       eapply wf_defs_updateAddAL; try solve [eauto | id_neq_pid_tac]
+      ]
+    ]
+  ]).
+Qed.
+
+(* go to infra *)
+Lemma getCmdID_in_getCmdsIDs : forall cs i0 c,
+  getCmdID c = Some i0 ->
+  In c cs ->
+  In i0 (getCmdsIDs cs).
+Proof.
+  induction cs; intros.
+    inv H0.
+
+    simpl in *.
+    destruct H0 as [H0 | H0]; subst.
+      rewrite H. simpl. auto.
+      
+      apply IHcs in H; auto.
+      destruct (getCmdID a); simpl; auto.
+Qed.
+
+(* go to infra *)
+Lemma getCmdID_in_getBlocksIDs : forall i0 c l0 ps0 cs0 tmn0,
+  getCmdID c = Some i0 ->
+  In c cs0 ->
+  In i0 (getBlockIDs (block_intro l0 ps0 cs0 tmn0)).
+Proof.
+  intros. 
+  simpl. 
+  apply in_or_app. right.
+  eapply getCmdID_in_getCmdsIDs; eauto.
+Qed.
+
+Lemma WF_PhiInfo_spec14: forall pinfo l1 ps1 cs11 t v align0 cs tmn2
+  (Hwfpi: WF_PhiInfo pinfo) (Huniq: uniqFdef (PI_f pinfo))
+  (HBinF: blockInFdefB (block_intro l1 ps1
+                 (cs11 ++ insn_alloca (PI_id pinfo) t v align0 :: cs) tmn2)
+               (PI_f pinfo) = true),
+  getEntryBlock (PI_f pinfo) =
+    ret block_intro l1 ps1
+         (cs11 ++ insn_alloca (PI_id pinfo) t v align0 :: cs) tmn2.
+Proof.
+  intros.
+  destruct Hwfpi as [Hwfpi _].
+  unfold promotable_alloca in Hwfpi.
+  inv_mbind. symmetry_ctx.
+  destruct b as [l0 ps0 cs0 tmn0].
+  f_equal.
+  eapply block_eq1 with (id0:=PI_id pinfo); eauto.
+    apply entryBlockInFdef in HeqR.
+    eapply inGetBlockIDs__lookupBlockViaIDFromFdef; eauto.
+    apply find_promotable_alloca_spec in Hwfpi.
+    destruct Hwfpi as [J _].
+    eapply getCmdID_in_getBlocksIDs; eauto. 
+      simpl; auto.
+
+    eapply getCmdID_in_getBlocksIDs; eauto using in_middle.
+      simpl; auto.
+Qed.
+
+(* go to infra *)
+Lemma uniqFdef_cmds_split_middle: forall (cs2 cs2' : list cmd) (c : cmd) 
+  (cs1 cs1' : list cmd) F l0 ps0 tmn0
+  (Huniq: uniqFdef F)
+  (HBinF: blockInFdefB (block_intro l0 ps0 (cs1 ++ c :: cs2) tmn0) F = true)
+  (H: cs1 ++ c :: cs2 = cs1' ++ c :: cs2'), cs1 = cs1' /\ cs2 = cs2'.
+Proof.
+  intros.
+  apply uniqFdef__blockInFdefB__nodup_cmds in HBinF; auto.
+  apply NoDup_cmds_split_middle in H; auto.
+Qed.
+
+Lemma WF_PhiInfo_spec15: forall (pinfo : PhiInfo) (tmn2 : terminator)
+  (lc2 : Opsem.GVsMap) (als2 : list mblock) (Hwfpi : WF_PhiInfo pinfo)
+  (B : block) (t : typ) (v : value)
+  (align0 : align) (EC : list Opsem.ExecutionContext) (cs : list cmd)
+  (Mem : mem) 
+  (Heq3 : exists l1 : l,
+           exists ps1 : phinodes,
+             exists cs11 : list cmd,
+               B =
+               block_intro l1 ps1
+                 (cs11 ++ insn_alloca (PI_id pinfo) t v align0 :: cs) tmn2)
+  (HBinF1 : blockInFdefB B (PI_f pinfo) = true)
+  (Hpalloca : wf_State pinfo
+               {|
+               Opsem.ECS := {|
+                            Opsem.CurFunction := PI_f pinfo;
+                            Opsem.CurBB := B;
+                            Opsem.CurCmds := insn_alloca 
+                                               (PI_id pinfo) t v align0 :: cs;
+                            Opsem.Terminator := tmn2;
+                            Opsem.Locals := lc2;
+                            Opsem.Allocas := als2 |} :: EC;
+               Opsem.Mem := Mem |})
+  (Huniq : uniqFdef (PI_f pinfo)),
+  lookupAL (GVsT DGVs) lc2 (PI_id pinfo) = merror.
+Proof.
+  intros.
+  destruct Hpalloca as [Hpalloca _].
+  destruct Heq3 as [l1 [ps1 [cs11 Heq3]]]; subst.
+  assert (getEntryBlock (PI_f pinfo) = 
+    Some 
+      (block_intro l1 ps1
+        (cs11 ++ insn_alloca (PI_id pinfo) t v align0 :: cs) tmn2))
+    as Hentry.
+    apply WF_PhiInfo_spec14; auto.
+  assert (G:=Hentry).
+  apply WF_PhiInfo_spec13 in G; auto.
+  destruct G as [A [B C]]; subst.
+  apply Hpalloca; simpl; auto.
+    unfold before_palloca.
+    fill_ctxhole.
+    intros.
+    assert (cs11 = cs1 /\ cs = cs3) as G.
+      eapply uniqFdef_cmds_split_middle; eauto.
+    destruct G; subst.
+    exists cs1. exists nil. auto.
+Qed.
+
+Lemma s_genInitState__palloca: forall S main VarArgs cfg IS pinfo
+  (Hwfpi: WF_PhiInfo pinfo) (Hwfs: wf_system S)
+  (Hinit : @Opsem.s_genInitState DGVs S main VarArgs Mem.empty = ret (cfg, IS)),
+  wf_State pinfo IS.
+Proof.
+  intros.
+  simpl_s_genInitState.
+  split; simpl; auto.
+    intros J1 J2 J3. simpl in *.
+    apply getParentOfFdefFromSystem__moduleInProductsInSystemB in HeqR0.
+    destruct HeqR0.
+    eapply arguments_dont_define_pid; eauto using wf_system__uniqFdef.
+Qed.
